Phi_Semantics/PhiSem_Base.thy
@@ -2,12 +2,6 @@ theory PhiSem_Base
   imports Phi_System.PhiSem_Formalization_Tools2
 begin
 
-
-type_synonym symbol = string \<comment> \<open>Right now we are using string directly which is very inefficient.
-  In future, we will instead use a global stateful symbol table that assigns each string dynamically
-  to a numeric index that is unique throughout the ML execution session.
-  The approach ensures semantic equity and, only takes logarithm space to the total number of symbols.
-\<close>
-type_synonym field_name = symbol
+(*TODO: remove this!*)
 
 end
