Phi_Semantics/PhiSem_Agg_Path_Machine_Int.thy
@@ -1,0 +1,5 @@
+theory PhiSem_Agg_Path_Machine_Int
+  imports PhiSem_Aggregate_Base
+begin
+
+end
